Day 9

Aoc2025/Util/Grid.lean
@@ -1,17 +1,44 @@
 import Aoc2025.Util.Coord
 import Batteries.Data.List.Lemmas
 
+abbrev FixedGrid (α : Type) (width height : Nat) :=
+  Vector (Vector α width) height
+
+namespace FixedGrid
+variable {α : Type} {width height : Nat} (grid : FixedGrid α width height)
+
+abbrev inBoundsXY (_grid : FixedGrid α width height) (x y : Int) :=
+  0 <= x ∧ x < width ∧ 0 <= y ∧ y < height
+abbrev inBounds (pos : Coord) :=
+  grid.inBoundsXY pos.x pos.y
+
+@[simp, grind =]
+instance : GetElem (FixedGrid α width height) Coord α inBounds where
+  getElem grid pos h := grid[pos.y.toNat][pos.x.toNat]
+
+-- Replace grid[pos] with (f grid[pos]), linearly.
+def modify? (pos : Coord) (f : α -> α) : FixedGrid α width height :=
+  let ⟨rows, hrows⟩ := grid
+  let rows' := ⟨rows.modify pos.y.toNat (fun ⟨row, hrow⟩ =>
+      ⟨row.modify pos.x.toNat f, (by grind)⟩),
+      (by grind)⟩
+  rows'
+
+-- Replace grid[pos] with value, linearly.
+def set? (pos : Coord) (value : α) : FixedGrid α width height :=
+  grid.modify? pos (fun _ => value)
+
+end FixedGrid
+
 structure Grid (α : Type) where
   width : Nat
   height : Nat
-  rows : Vector (Vector α width) height
+  rows : FixedGrid α width height
 deriving DecidableEq, Inhabited, Repr
 
 namespace Grid
-
 variable {α : Type} (grid : Grid α)
 
-instance : Inhabited (Grid α) := ⟨⟨0, 0, #v[]⟩⟩
 instance : ∀ [ToString α], ToString (Grid α) where
   toString grid :=
     ("\n".intercalate ·.toList) <|
@@ -78,19 +105,40 @@ instance : GetElem (Grid α) Coord α inBounds where
 
 -- Replace grid[pos] with (f grid[pos]), linearly.
 def modify? (pos : Coord) (f : α -> α) : Grid α :=
-  let ⟨width, height, ⟨rows, hrows⟩⟩ := grid
-  let rows' := ⟨rows.modify pos.y.toNat (fun ⟨row, hrow⟩ =>
-      ⟨row.modify pos.x.toNat f, (by grind)⟩),
-      (by grind)⟩
-  Grid.mk width height rows'
+  Grid.mk grid.width grid.height (grid.rows.modify? pos f)
+
+@[simp, grind =]
+theorem modify?_width {grid : Grid α} {pos : Coord} {f : α -> α}
+  : (modify? grid pos f).width = grid.width := by
+  simp [modify?]
+
+@[simp, grind =]
+theorem modify?_height {grid : Grid α} {pos : Coord} {f : α -> α}
+  : (modify? grid pos f).height = grid.height := by
+  simp [modify?]
+
+@[simp, grind =]
+theorem modify?_inBounds {grid : Grid α} {pos : Coord} {f : α -> α}
+  : (grid.modify? pos f).inBounds pos ↔ grid.inBounds pos := by
+  simp
 
 -- Replace grid[pos] with value, linearly.
 def set? (pos : Coord) (value : α) : Grid α :=
   grid.modify? pos (fun _ => value)
 
 @[simp, grind =]
-theorem modify?_inBounds {grid : Grid α} {pos : Coord} {f : α -> α}
-  : (grid.modify? pos f).inBounds pos ↔ grid.inBounds pos := by
-  unfold modify? ; simp
+theorem set?_width {grid : Grid α} {pos : Coord} {x : α}
+  : (set? grid pos x).width = grid.width := by
+  simp [set?]
+
+@[simp, grind =]
+theorem set?_height {grid : Grid α} {pos : Coord} {x : α}
+  : (set? grid pos x).height = grid.height := by
+  simp [set?]
+
+@[simp, grind =]
+theorem set?_inBounds {grid : Grid α} {pos : Coord} {x : α}
+  : (grid.set? pos x).inBounds pos ↔ grid.inBounds pos := by
+  simp
 
 end Grid
