Aoc2025/Day09.lean
@@ -1,0 +1,165 @@
+import Aoc2025.Util
+
+namespace Day09
+open Day09
+
+def parseInput : IO (Array Coord) := do
+  let stdin <- IO.getStdin
+  let lines <- stdin.lines
+  let coords <- lines.mapM (fun line => do
+    let components := line.splitOn ","
+    match <- components.mapM String.toIntIO with
+    | [x, y] => pure <| Coord.mk x y
+    | _ => throw <| IO.userError s!"Bad coordinate: {line}")
+  return coords
+
+def allRects (pts : Array Coord) : List (Nat × Fin pts.size × Fin pts.size) := Id.run do
+  let rects := List.range pts.size
+    |>.mapRevMem (fun a ha =>
+      let ptA := pts[a]'(by grind)
+      Task.spawn fun () =>
+        List.range' (a + 1) (pts.size - (a + 1))
+          |>.mapRevMem (fun b hb =>
+            let ptB := pts[b]'(by grind)
+            (((ptA - ptB).abs + (.down + .right)).area.natAbs,
+             Fin.mk (n:=pts.size) a (by grind),
+             Fin.mk (n:=pts.size) b (by grind)))
+          |>.mergeSort (·.1 ≥ ·.1))
+    |>.parallelFold (List.merge · · (·.1 ≥ ·.1)) []
+  return rects.get
+
+def part1 (pts : Array Coord) : Id Nat := do
+  let rects := allRects pts
+  return if h : rects = [] then 0 else (rects.head h).1
+
+def countPrecedingEdges (edges : Array (Coord × Coord)) (pt : Coord) : IO Nat := do
+  let mut cnt := 0
+  let mut prevHalfEdgeRight : Option (Bool × Nat) := .none
+  for (eA, eB) in edges do
+    if eA.y > pt.y then break
+    if ¬(eA.x ≤ pt.x ∧ pt.x ≤ eB.x) then continue else
+    let thisHalfEdgeRight : Option (Bool × Nat) :=
+      if eA.x = pt.x then .some (true, cnt)
+      else if eB.x = pt.x then .some (false, cnt)
+      else .none
+    match prevHalfEdgeRight, thisHalfEdgeRight with
+    -- #---# (ordinary edge)
+    | .none, .none =>
+      prevHalfEdgeRight := .none
+      if eA.y = pt.y
+      then if 2 ∣ cnt then cnt := cnt + 1
+      else cnt := cnt + 1
+    /- --#    #--
+         | OR |
+       --#    #-- -/
+    | .some (false, n), .some (false, _)
+    | .some (true, n), .some (true, _) =>
+      prevHalfEdgeRight := .none
+      if eA.y ≠ pt.y then
+        -- If we are inside only thanks to this side edge, then we are
+        -- no longer inside.
+        if 2 ∣ n then cnt := cnt + 1
+    /- --#        #--
+         |   OR   |
+         #--    --# -/
+    | .some (false, n), .some (true, _)
+    | .some (true, n), .some (false, _) =>
+      prevHalfEdgeRight := .none
+      if eA.y ≠ pt.y then
+        -- We have crossed an edge
+        cnt := n + 1
+    -- Start of any of the above
+    | .none, .some (_, _) =>
+      prevHalfEdgeRight := thisHalfEdgeRight
+      -- No matter what, we stay in/enter the green tiles
+      if 2 ∣ cnt then cnt := cnt + 1
+    -- Should not really happen
+    | .some _, .none => prevHalfEdgeRight := .none
+  return cnt
+
+def makeEdge : Coord -> Coord -> Coord × Coord
+  | ⟨x1, y1⟩, ⟨x2, y2⟩ =>
+    (Coord.mk (min x1 x2) (min y1 y2),
+     Coord.mk (max x1 x2) (max y1 y2))
+
+def pointsToEdges (pts : Array Coord) : Array (Coord × Coord) :=
+  List.range pts.size
+    |>.mapRevMem (fun i hi0 =>
+    have hi : i < pts.size := by grind
+    let j := (i + 1) % pts.size
+    have hj : j < pts.size := Nat.mod_lt _ (by grind)
+    makeEdge pts[i] pts[j])
+    |>.toArray
+
+def partitionEdges (edges : Array (Coord × Coord)) : Array (Coord × Coord) × Array (Coord × Coord) :=
+  let horizEdges := edges.filter (fun (ptA, ptB) => ptA.y = ptB.y) |>.qsort (·.1.y < ·.1.y)
+  let vertEdges := edges.filter (fun (ptA, ptB) => ptA.x = ptB.x) |>.qsort (·.1.x < ·.1.x)
+                   |>.map (fun (ptA, ptB) => (ptA.transpose, ptB.transpose))
+  (horizEdges, vertEdges)
+
+def testEdges (pts : Array Coord) (tests : Array Coord) : IO (Array Nat) := do
+  tests.mapM (countPrecedingEdges (pointsToEdges pts |> partitionEdges |>.1) ·)
+
+/- #-#
+   | |
+   #-# -/
+def testE1 : Array Coord := #[⟨0, 0⟩, ⟨2, 0⟩, ⟨2, 2⟩, ⟨0, 2⟩]
+-- #eval testEdges testE1 #[⟨0, -1⟩, ⟨0, 0⟩, ⟨1, 1⟩, ⟨2, 2⟩, ⟨2, 3⟩]
+/- #-#
+   | |
+   | #-#
+   |   |
+   #---# -/
+def testE2 : Array Coord := #[⟨0, 0⟩, ⟨2, 0⟩, ⟨2, 2⟩, ⟨4, 2⟩, ⟨4, 4⟩, ⟨0, 4⟩]
+-- #eval testEdges testE2 #[⟨0, 0⟩, ⟨1, 2⟩, ⟨1, 4⟩, ⟨1, 5⟩]
+-- #eval testEdges testE2 #[⟨2, 3⟩, ⟨3, 1⟩, ⟨3, 2⟩, ⟨3, 4⟩]
+-- #eval testEdges testE2 #[⟨3, 5⟩, ⟨4, 0⟩, ⟨4, 2⟩, ⟨4, 3⟩, ⟨4, 5⟩]
+/- #---#
+   |   |
+   | #-#
+   | |
+   #-#   -/
+def testE3 : Array Coord := #[⟨0, 0⟩, ⟨4, 0⟩, ⟨4, 2⟩, ⟨2, 2⟩, ⟨2, 4⟩, ⟨0, 4⟩]
+-- #eval testEdges testE3 #[⟨0, 3⟩, ⟨3, 2⟩, ⟨3, 3⟩, ⟨4, 2⟩, ⟨4, 3⟩]
+-- #eval testEdges testE3 #[⟨2, 2⟩, ⟨2, 3⟩, ⟨2, 4⟩, ⟨2, 5⟩]
+/- #-----#
+   |     |
+   #-# #-#
+     | |
+   #-# #-#
+   |     |
+   #-----# -/
+def testE4 : Array Coord := #[⟨0, 0⟩, ⟨6, 0⟩, ⟨6, 2⟩, ⟨4, 2⟩, ⟨4, 4⟩, ⟨6, 4⟩, ⟨6, 6⟩,
+  ⟨0, 6⟩, ⟨0, 4⟩, ⟨2, 4⟩, ⟨2, 2⟩, ⟨0, 2⟩]
+-- #eval testEdges testE4 #[⟨0, 0⟩, ⟨0, 2⟩, ⟨0, 3⟩, ⟨0, 4⟩, ⟨0, 6⟩, ⟨0, 7⟩]
+-- #eval testEdges testE4 #[⟨1, 0⟩, ⟨1, 2⟩, ⟨1, 3⟩, ⟨1, 4⟩, ⟨1, 6⟩, ⟨1, 7⟩]
+-- #eval testEdges testE4 #[⟨2, 0⟩, ⟨2, 2⟩, ⟨2, 3⟩, ⟨2, 5⟩, ⟨2, 6⟩, ⟨2, 7⟩]
+-- #eval testEdges testE4 #[⟨5, 0⟩, ⟨5, 2⟩, ⟨5, 3⟩, ⟨5, 4⟩, ⟨5, 6⟩, ⟨5, 7⟩]
+
+def part2 (pts : Array Coord) : IO Nat := do
+  let rects := allRects pts
+  let edges := pointsToEdges pts
+  let (horizEdges, vertEdges) := partitionEdges edges
+  let countEdges (pt : Coord) := do
+    return (<- countPrecedingEdges horizEdges pt,
+            <- countPrecedingEdges vertEdges pt.transpose)
+
+  let rectInBounds (ptA ptB : Coord) : IO Bool := do
+    let edgesA <- countEdges ptA
+    let edgesB <- countEdges ptB
+    let edgesAB <- countEdges ⟨ptA.x, ptB.y⟩
+    let edgesBA <- countEdges ⟨ptB.x, ptA.y⟩
+    return edgesA.1 = edgesAB.1 ∧ edgesA.2 = edgesBA.2 ∧
+      edgesB.1 = edgesBA.1 ∧ edgesB.2 = edgesAB.2
+
+  return match <- rects.findM? (fun (_, a, b) => rectInBounds pts[a] pts[b]) with
+  | .some (size, _, _) => size
+  | .none => 0
+
+end Day09
+open Day09
+
+def main : IO Unit := do
+  let input <- parseInput
+  IO.println s!"Part 1: {<- part1 input}"
+  IO.println s!"Part 2: {<- part2 input}"
