Aoc2025/Util.lean
@@ -2,3 +2,4 @@ import Aoc2025.Util.Parse
 import Aoc2025.Util.Coord
 import Aoc2025.Util.Grid
 import Aoc2025.Util.Interval
+import Aoc2025.Util.Misc
