Aoc2025/Util/Misc.lean
@@ -1,0 +1,37 @@
+namespace List
+
+universe u v
+variable {α : Type u} {β : Type v}
+
+@[specialize]
+def mapRevMem (xs : List α) (f : (x : α) -> x ∈ xs -> β) (tail : List β := []) : List β :=
+  match xs with
+  | [] => tail
+  | x :: xs' => mapRevMem xs'
+    (fun y h => f y (h.tail x))
+    (f x (.head _) :: tail)
+
+def mapMem (xs : List α) (f : (x : α) -> x ∈ xs -> β) : List β :=
+  xs.mapRevMem f |>.reverse
+
+def parallelFoldOnceRev 
+  (f : α -> α -> α)
+  (xs : List (Task α))
+  (tail : List (Task α) := [])
+  : List (Task α) :=
+  match xs with
+  | [] => tail
+  | [x] => x :: tail
+  | x::y::xs' =>
+    parallelFoldOnceRev f xs'
+    ((x.bind fun x => y.map fun y => f x y) :: tail)
+
+def parallelFold (f : α -> α -> α) (identity : α) (xs : List (Task α)) : Task α :=
+  let rec loop fuel xs :=
+    match fuel, xs with
+    | _, [] | 0, _ => Task.pure identity
+    | _, [x] => x
+    | fuel + 1, _ => loop fuel (parallelFoldOnceRev f xs)
+  loop (xs.length * xs.length) xs
+
+end List
